theories/Multicore/Common/MigrationFacts.v
@@ -1,0 +1,46 @@
+From Stdlib Require Import Arith Lia.
+From RocqSched Require Import Foundation.Base.
+From RocqSched Require Import Semantics.Schedule.
+From RocqSched Require Import Multicore.Common.MultiCoreBase.
+From RocqSched Require Import Multicore.Common.Admissibility.
+From RocqSched Require Import Multicore.Common.PlacementFacts.
+
+(** Abstract migration between two consecutive slots. *)
+Definition migrates_between
+    (sched : Schedule) (j : JobId) (t : Time) (c1 c2 : CPU) : Prop :=
+  c1 <> c2 /\
+  sched t c1 = Some j /\
+  sched (S t) c2 = Some j.
+
+Lemma migration_respects_admissibility :
+  forall adm m sched j t c1 c2,
+    schedule_respects_admissibility adm m sched ->
+    c1 < m ->
+    c2 < m ->
+    migrates_between sched j t c1 c2 ->
+    adm j c1 /\ adm j c2.
+Proof.
+  intros adm m sched j t c1 c2 Hrespect Hc1 Hc2 [_ [Hrun1 Hrun2]].
+  split.
+  - eapply running_on_admissible_cpu; eauto.
+  - eapply running_on_admissible_cpu; eauto.
+Qed.
+
+Lemma singleton_respect_prevents_cross_cpu_migration :
+  forall assign m sched j t c1 c2,
+    schedule_respects_admissibility (singleton_admissibility assign) m sched ->
+    c1 < m ->
+    c2 < m ->
+    sched t c1 = Some j ->
+    sched (S t) c2 = Some j ->
+    c1 = c2.
+Proof.
+  intros assign m sched j t c1 c2 Hrespect Hc1 Hc2 Hrun1 Hrun2.
+  pose proof
+    (singleton_schedule_respects_implies_assigned_cpu
+       assign m sched j t c1 Hrespect Hc1 Hrun1) as Hass1.
+  pose proof
+    (singleton_schedule_respects_implies_assigned_cpu
+       assign m sched j (S t) c2 Hrespect Hc2 Hrun2) as Hass2.
+  congruence.
+Qed.
